theories/gitree/reify.v
@@ -16,241 +16,9 @@ Section reifiers.
       sReifier_cofe X (HX : Cofe X) :: Cofe (sReifier_state ♯ X);
     }.
 
-  (** Global reifiers: a collection of reifiers *)
-  Inductive gReifiers : nat → Type :=
-  | gReifiers_nil : gReifiers 0
-  | gReifiers_cons {n} : sReifier → gReifiers n → gReifiers (S n)
-  .
-
-  Definition grs_S_inv {n} (P : gReifiers (S n) → Type)
-    (Hcons : ∀ sR v, P (gReifiers_cons sR v)) v : P v.
-  Proof.
-    revert P Hcons.
-    refine match v with gReifiers_nil => tt
-                      | gReifiers_cons sR v => λ P Hcons, Hcons sR v end.
-  Defined.
-
-  #[global] Instance gReifiers_lookup_total : ∀ m, LookupTotal (fin m) sReifier (gReifiers m) :=
-  fix go m i {struct i} := let _ : ∀ m, LookupTotal _ _ _ := @go in
-  match i in fin m return gReifiers m → sReifier with
-  | 0%fin => grs_S_inv (λ _, sReifier) (λ x _, x)
-  | FS j => grs_S_inv (λ _, sReifier) (λ _ v, v !!! j)
-  end.
-
-  Program Definition gReifiers_ops {n} (rs : gReifiers n) : opsInterp :=
-    {| opid := { i : fin n & opid (sReifier_ops (rs !!! i)) };
-       opsInterp_lookup := λ iop, sReifier_ops (rs !!! projT1 iop) (projT2 iop)
-    |}.
-  Next Obligation.
-    intros n rs.
-    unfold EqDecision. intros [i1 x1] [i2 x2].
-    unfold Decision.
-    destruct (decide (i1 = i2)) as [<-|Hi].
-    - destruct (decide (x1 = x2)) as [<-|Hx].
-      + left. reflexivity.
-      + right. naive_solver.
-    - right. naive_solver.
-  Qed.
-
-  Fixpoint gReifiers_state {n} (rs : gReifiers n) : oFunctor :=
-    match rs with
-    | gReifiers_nil => unitO
-    | gReifiers_cons sR rs => sReifier_state sR * (gReifiers_state rs)
-    end.
-
-  #[export] Instance reifiers_state_cofe {n} (rs : gReifiers n) X `{!Cofe X} :
-    Cofe (gReifiers_state rs ♯ X).
-  Proof.
-    induction rs; simpl; first apply _.
-    destruct s. apply _.
-  Qed.
-  #[export] Instance reifiers_state_inhab {n} (rs : gReifiers n) :
-    Inhabited (gReifiers_state rs ♯ unitO).
-  Proof.
-    induction rs; simpl; first apply _.
-    destruct s. apply _.
-  Qed.
-
-  Fixpoint gState_rest {m} (i : fin m) : gReifiers m → oFunctor :=
-    match i in fin m return gReifiers m → oFunctor with
-    | 0%fin => grs_S_inv (λ _, oFunctor)
-                 (λ sR rs, gReifiers_state rs)
-    | FS j => grs_S_inv (λ _, oFunctor)
-                 (λ sR rs, sReifier_state sR * gState_rest j rs)%OF
-    end.
-
-  Lemma gState_decomp' {m} (i : fin m) (rs : gReifiers m) {X} `{!Cofe X} :
-    ofe_iso (gReifiers_state rs ♯ X)
-            ((sReifier_state (rs !!! i) ♯ X) * (gState_rest i rs ♯ X))%type.
-  Proof.
-    revert i. induction rs as [|n r rs]=>i.
-    { inversion i. }
-    inv_fin i; simpl.
-    { apply iso_ofe_refl. }
-    intros i.
-    specialize (IHrs i).
-    unshelve esplit.
-    - simple refine (λne xr, let sr := ofe_iso_1 IHrs (xr.2) in
-                             (sr.1,(xr.1,sr.2))).
-      solve_proper.
-    - simple refine (λne sxr, let r' := ofe_iso_2 IHrs (sxr.1,sxr.2.2) in
-                              (sxr.2.1, r')).
-      solve_proper.
-    - intros (s & x & rest). simpl. repeat f_equiv; rewrite ofe_iso_12//.
-    - intros (x & rest). simpl. f_equiv.
-      rewrite -surjective_pairing. apply ofe_iso_21.
-  Defined.
-  Definition gState_decomp {m} (i : fin m) {rs : gReifiers m} {X} `{!Cofe X} :
-    (gReifiers_state rs ♯ X) -n> ((sReifier_state (rs !!! i) ♯ X) * (gState_rest i rs ♯ X))%type
-    := ofe_iso_1 (gState_decomp' i rs).
-  Program Definition gState_recomp {m} {i : fin m} {rs : gReifiers m} {X} `{!Cofe X} :
-    (gState_rest i rs ♯ X) -n> (sReifier_state (rs !!! i) ♯ X) -n> (gReifiers_state rs ♯ X)
-    := λne rest st, ofe_iso_2 (gState_decomp' i rs) (st, rest).
-  Solve All Obligations with solve_proper_please.
-
-  Lemma gState_decomp_recomp {m} (i : fin m) {rs : gReifiers m} {X} `{!Cofe X}
-    (σ : sReifier_state (rs !!! i) ♯ X) rest :
-    gState_decomp i (gState_recomp rest σ) ≡ (σ, rest).
-  Proof. rewrite ofe_iso_12. reflexivity. Qed.
-  Lemma gState_recomp_decomp {m} (i : fin m) {rs : gReifiers m} {X} `{!Cofe X}
-    (σ : sReifier_state (rs !!! i) ♯ X) rest fs :
-      gState_decomp i fs ≡ (σ, rest) →
-      gState_recomp rest σ ≡ fs.
-  Proof.
-    unfold gState_recomp. simpl.
-    intros <-. rewrite ofe_iso_21//.
-  Qed.
-  Opaque gState_recomp gState_decomp.
-
-  Program Definition gReifiers_re {n} (rs : gReifiers n) {X} `{!Cofe X}
-    (op : opid (gReifiers_ops rs)) :
-    (Ins (gReifiers_ops rs op) ♯ X) * (gReifiers_state rs ♯ X) -n>
-      optionO ((Outs (gReifiers_ops rs op) ♯ X) * (gReifiers_state rs ♯ X))
-    :=  λne xst,
-      let  i := projT1 op in
-      let op' := projT2 op in
-      let x := xst.1 in
-      let st := xst.2 in
-      let fs := gState_decomp i st in
-      let σ := fs.1 in
-      let rest := fs.2 in
-      let rx := sReifier_re (rs !!! i) op' (x, σ) in
-      optionO_map (prodO_map idfun (gState_recomp rest)) rx.
-  Next Obligation. solve_proper_please. Qed.
-
-  (** We can turn a collection of reifiers into a single reifier *)
-  Definition gReifiers_sReifier {n} (rs : gReifiers n) : sReifier :=
-    {| sReifier_ops := gReifiers_ops rs;
-       sReifier_state := gReifiers_state rs;
-       sReifier_re := @gReifiers_re n rs;
-    |}.
-
-  Lemma gReifiers_re_idx {n}  (i : fin n) (rs : gReifiers n)
-    {X} `{!Cofe X} (op : opid (sReifier_ops (rs !!! i)))
-    (x : Ins (sReifier_ops _ op) ♯ X)
-    (σ : sReifier_state (rs !!! i) ♯ X) (rest : gState_rest i rs ♯ X) :
-    gReifiers_re rs (existT i op) (x, gState_recomp rest σ) ≡
-      optionO_map (prodO_map idfun (gState_recomp rest))
-           (sReifier_re (rs !!! i) op (x,σ)).
-  Proof.
-    unfold gReifiers_re. cbn-[prodO_map optionO_map].
-    f_equiv; last repeat f_equiv.
-    - eapply optionO_map_proper.
-      intros [x1 x2]; simpl. f_equiv.
-      f_equiv. f_equiv.
-      rewrite gState_decomp_recomp//.
-    - rewrite gState_decomp_recomp//.
-  Qed.
-
-  Class subReifier {n} (r : sReifier) (rs : gReifiers n) :=
-    { sR_idx : fin n;
-      sR_ops :: subEff (sReifier_ops r) (sReifier_ops (rs !!! sR_idx));
-      sR_state  {X} `{!Cofe X} :
-        ofe_iso (sReifier_state r ♯ X) (sReifier_state (rs !!! sR_idx) ♯ X);
-      sR_re m {X} `{!Cofe X} (op : opid (sReifier_ops r))
-        (x : Ins (sReifier_ops _ op) ♯ X)
-        (y : Outs (sReifier_ops _ op) ♯ X)
-        (s1 s2 : sReifier_state r ♯ X) :
-        sReifier_re r op (x, s1) ≡{m}≡ Some (y, s2) →
-        sReifier_re (rs !!! sR_idx) (subEff_opid op)
-          (subEff_conv_ins x, ofe_iso_1 sR_state s1) ≡{m}≡
-          Some (subEff_conv_outs y, ofe_iso_1 sR_state s2) }.
-
-  #[global] Instance subReifier_here {n} (r : sReifier) (rs : gReifiers n) :
-    subReifier r (gReifiers_cons r rs).
-  Proof.
-    simple refine ({| sR_idx := 0%fin |}).
-    - simpl. intros. apply iso_ofe_refl.
-    - intros X ? op x y s1 s2.
-      simpl. eauto.
-  Defined.
-  #[global] Instance subReifier_there {n} (r r' : sReifier) (rs : gReifiers n) :
-    subReifier r rs →
-    subReifier r (gReifiers_cons r' rs).
-  Proof.
-    intros SR.
-    simple refine ({| sR_idx := FS sR_idx |}).
-    - simpl. intros. apply sR_state.
-    - intros X ? op x y s1 s2.
-      simpl. apply sR_re.
-  Defined.
-
-  #[local] Definition subR_op {n} {r : sReifier} {rs : gReifiers n} `{!subReifier r rs} :
-    opid (sReifier_ops r) → opid (gReifiers_ops rs).
-  Proof.
-    intros op.
-    simpl.
-    refine (existT sR_idx (subEff_opid op)).
-  Defined.
-  Definition subR_conv_state {n} {r : sReifier} {rs : gReifiers n} `{!subReifier r rs}
-    {X} `{!Cofe X}:
-    (sReifier_state r ♯ X) -n> (sReifier_state (rs !!! sR_idx) ♯ X) :=
-    ofe_iso_1 sR_state.
-  #[export] Instance subReifier_subEff {n} {r : sReifier} {rs : gReifiers n} `{!subReifier r rs} :
-    subEff (sReifier_ops r) (gReifiers_ops rs).
-  Proof.
-    simple refine {| subEff_opid := subR_op |}.
-    - intros op X ?. simpl.
-      apply subEff_ins.
-    - intros op X ?. simpl.
-      apply subEff_outs.
-  Defined.
-
-  Lemma subReifier_reify_idx {n} (r : sReifier) (rs : gReifiers n)
-    `{!subReifier r rs} {X} `{!Cofe X} (op : opid (sReifier_ops r))
-    (x : Ins (sReifier_ops _ op) ♯ X)
-    (y : Outs (sReifier_ops _ op) ♯ X)
-    (s1 s2 : sReifier_state r ♯ X) :
-        sReifier_re r op (x, s1) ≡ Some (y, s2) →
-        sReifier_re (rs !!! sR_idx) (subEff_opid op)
-          (subEff_conv_ins x, ofe_iso_1 sR_state s1) ≡
-          Some (subEff_conv_outs y, ofe_iso_1 sR_state s2).
-  Proof.
-    intros Hx. apply equiv_dist=>m.
-    apply sR_re. by apply equiv_dist.
-  Qed.
-
-  Lemma subReifier_reify {n} (r : sReifier)
-    (rs : gReifiers n) `{!subReifier r rs} {X} `{!Cofe X}
-    (op : opid (sReifier_ops r))
-    (x : Ins (sReifier_ops _ op) ♯ X) (y : Outs (sReifier_ops _ op) ♯ X)
-    (σ σ' : sReifier_state r ♯ X) (rest : gState_rest sR_idx rs ♯ X) :
-    sReifier_re r op (x,σ) ≡ Some (y, σ') →
-    gReifiers_re rs (subEff_opid op)
-      (subEff_conv_ins x, gState_recomp rest (subR_conv_state σ))
-      ≡ Some (subEff_conv_outs y, gState_recomp rest (subR_conv_state σ')).
-  Proof.
-    intros Hre.
-    eapply subReifier_reify_idx in Hre.
-    rewrite gReifiers_re_idx//.
-    rewrite Hre. simpl. reflexivity.
-  Qed.
-
-  (************************************************************************)
-
-  Context {n : nat} (rs : gReifiers n).
-  Notation F := (gReifiers_ops rs).
-  Notation stateF := (gReifiers_state rs).
+  Context (r : sReifier).
+  Notation F := (sReifier_ops r).
+  Notation stateF := (sReifier_state r).
   Notation IT := (IT F).
   Notation ITV := (ITV F).
   Implicit Type op : opid F.
@@ -282,7 +50,7 @@ Section reifiers.
   Proof.
     simpl.
     simple refine (λne i (k : _ -n> _) (s : stateF ♯ IT), _).
-    - simple refine (let ns := gReifiers_re rs op (oFunctor_map _ (inlO,fstO) i, s) in _).
+    - simple refine (let ns := sReifier_re r op (oFunctor_map _ (inlO,fstO) i, s) in _).
       simple refine (from_option (λ ns,
                          let out2' := k $ oFunctor_map (Outs (F op)) (fstO,inlO) ns.1 in
                          (ns.2, Tau $ laterO_map fstO out2'))
@@ -337,7 +105,7 @@ Section reifiers.
   Qed.
 
   Lemma reify_vis_dist m op i o k σ σ' :
-    gReifiers_re rs op (i,σ) ≡{m}≡ Some (o,σ') →
+    sReifier_re r op (i,σ) ≡{m}≡ Some (o,σ') →
     reify (Vis op i k) σ ≡{m}≡ (σ', Tau $ k o).
   Proof.
     intros Hst.
@@ -347,16 +115,16 @@ Section reifiers.
              σ).
     { f_equiv. rewrite IT_rec1_vis//. }
     Opaque prod_in. simpl.
-    pose (r := (gReifiers_re rs op
+    pose (rs := (sReifier_re r op
       (oFunctor_map (Ins (F op)) (inlO, fstO)
                     (oFunctor_map (Ins (F op)) (sumO_rec idfun unreify, prod_in idfun reify) i), σ))).
-    fold r.
-    assert (r ≡ gReifiers_re rs op (i,σ)) as Hr'.
-    { unfold r. f_equiv. f_equiv.
+    fold rs.
+    assert (rs ≡ sReifier_re r op (i,σ)) as Hr'.
+    { unfold rs. f_equiv. f_equiv.
       rewrite -oFunctor_map_compose.
       etrans; last by apply oFunctor_map_id.
       repeat f_equiv; intro; done. }
-    assert (r ≡{m}≡ Some (o,σ')) as Hr.
+    assert (rs ≡{m}≡ Some (o,σ')) as Hr.
     { by rewrite Hr' Hst. }
     trans (from_option (λ ns,
        (ns.2,
@@ -382,7 +150,7 @@ Section reifiers.
   Qed.
 
   Lemma reify_vis_eq op i o k σ σ' :
-    gReifiers_re rs op (i,σ) ≡ Some (o,σ') →
+    sReifier_re r op (i,σ) ≡ Some (o,σ') →
     reify (Vis op i k) σ ≡ (σ', Tau $ k o).
   Proof.
     intros H. apply equiv_dist=>m.
@@ -391,7 +159,7 @@ Section reifiers.
   Qed.
 
   Lemma reify_vis_None op i k σ :
-    gReifiers_re rs op (i,σ) ≡ None →
+    sReifier_re r op (i,σ) ≡ None →
     reify (Vis op i k) σ ≡ (σ, Err RuntimeErr).
   Proof.
     intros Hs.
@@ -402,16 +170,16 @@ Section reifiers.
     { f_equiv.
       apply IT_rec1_vis. }
     simpl.
-    pose (r := (gReifiers_re rs op
+    pose (rs := (sReifier_re r op
       (oFunctor_map (Ins (F op)) (inlO, fstO)
                     (oFunctor_map (Ins (F op)) (sumO_rec idfun unreify, prod_in idfun reify) i), σ))).
-    fold r.
-    assert (r ≡ gReifiers_re rs op (i,σ)) as Hr'.
-    { unfold r. f_equiv. f_equiv.
+    fold rs.
+    assert (rs ≡ sReifier_re r op (i,σ)) as Hr'.
+    { unfold rs. f_equiv. f_equiv.
       rewrite -oFunctor_map_compose.
       etrans; last by apply oFunctor_map_id.
       repeat f_equiv; intro; done. }
-    assert (r ≡ None) as Hr.
+    assert (rs ≡ None) as Hr.
     { by rewrite Hr' Hs. }
     trans (from_option (λ ns,
        (ns.2,
@@ -431,7 +199,7 @@ Section reifiers.
     (reify (Vis op i k1) σ1 ≡ (σ2, Tick β) ⊢
      reify (Vis op i (laterO_map k2 ◎ k1)) σ1 ≡ (σ2, Tick (k2 β)) : PROP)%I.
   Proof.
-    destruct (gReifiers_re rs op (i,σ1)) as [[o σ2']|] eqn:Hre; last first.
+    destruct (sReifier_re r op (i,σ1)) as [[o σ2']|] eqn:Hre; last first.
     - rewrite reify_vis_None; last by rewrite Hre//.
       iIntros "Hr". iExFalso.
       iPoseProof (prod_equivI with "Hr") as "[_ Hk]".
@@ -454,7 +222,7 @@ Section reifiers.
      ⊢ ∃ α, reify (Vis op i k1) σ1 ≡ (σ2, Tick α) ∧ ▷ (β ≡ k2 α)
       : PROP)%I.
   Proof.
-    destruct (gReifiers_re rs op (i,σ1)) as [[o σ2']|] eqn:Hre; last first.
+    destruct (sReifier_re r op (i,σ1)) as [[o σ2']|] eqn:Hre; last first.
     - rewrite reify_vis_None; last by rewrite Hre//.
       iIntros "Hr". iExFalso.
       iPoseProof (prod_equivI with "Hr") as "[_ Hk]".
@@ -484,7 +252,7 @@ Section reifiers.
   Lemma reify_is_always_a_tick op x k σ β σ' :
     reify (Vis op x k) σ ≡ (σ', β) → (∃ β', β ≡ Tick β') ∨ (β ≡ Err RuntimeErr).
   Proof.
-    destruct (gReifiers_re rs op (x, σ)) as [[o σ'']|] eqn:Hre; last first.
+    destruct (sReifier_re r op (x, σ)) as [[o σ'']|] eqn:Hre; last first.
     - rewrite reify_vis_None; last by rewrite Hre//.
       intros [_ ?]. by right.
     - rewrite reify_vis_eq;last by rewrite Hre.
@@ -496,4 +264,4 @@ Section reifiers.
   Qed.
 
 End reifiers.
-Arguments reify {n} rs.
+
