theories/gitree.v
@@ -1,4 +1,4 @@
 From iris.proofmode Require Export base tactics classes.
 From iris.base_logic.lib Require Export own fancy_updates invariants.
 From gitrees Require Export prelude.
-From gitrees.gitree Require Export core reify reductions weakestpre lambda.
+From gitrees.gitree Require Export core reify greifiers reductions weakestpre lambda.
