theories/gitree/greifiers.v
@@ -1,0 +1,284 @@
+From iris.proofmode Require Import classes tactics.
+From iris.base_logic.lib Require Export invariants.
+From gitrees Require Import prelude.
+From gitrees.gitree Require Import core reify.
+
+
+Section greifiers.
+  #[local] Open Scope type.
+
+    (** Global reifiers: a collection of reifiers *)
+  Inductive gReifiers : nat → Type :=
+  | gReifiers_nil : gReifiers 0
+  | gReifiers_cons {n} : sReifier → gReifiers n → gReifiers (S n)
+  .
+
+  Definition grs_S_inv {n} (P : gReifiers (S n) → Type)
+    (Hcons : ∀ sR v, P (gReifiers_cons sR v)) v : P v.
+  Proof.
+    revert P Hcons.
+    refine match v with gReifiers_nil => tt
+                      | gReifiers_cons sR v => λ P Hcons, Hcons sR v end.
+  Defined.
+
+  #[global] Instance gReifiers_lookup_total : ∀ m, LookupTotal (fin m) sReifier (gReifiers m) :=
+  fix go m i {struct i} := let _ : ∀ m, LookupTotal _ _ _ := @go in
+  match i in fin m return gReifiers m → sReifier with
+  | 0%fin => grs_S_inv (λ _, sReifier) (λ x _, x)
+  | FS j => grs_S_inv (λ _, sReifier) (λ _ v, v !!! j)
+  end.
+
+  Program Definition gReifiers_ops {n} (rs : gReifiers n) : opsInterp :=
+    {| opid := { i : fin n & opid (sReifier_ops (rs !!! i)) };
+       opsInterp_lookup := λ iop, sReifier_ops (rs !!! projT1 iop) (projT2 iop)
+    |}.
+  Next Obligation.
+    intros n rs.
+    unfold EqDecision. intros [i1 x1] [i2 x2].
+    unfold Decision.
+    destruct (decide (i1 = i2)) as [<-|Hi].
+    - destruct (decide (x1 = x2)) as [<-|Hx].
+      + left. reflexivity.
+      + right. naive_solver.
+    - right. naive_solver.
+  Qed.
+
+  Fixpoint gReifiers_state {n} (rs : gReifiers n) : oFunctor :=
+    match rs with
+    | gReifiers_nil => unitO
+    | gReifiers_cons sR rs => sReifier_state sR * (gReifiers_state rs)
+    end.
+
+  #[export] Instance reifiers_state_cofe {n} (rs : gReifiers n) X `{!Cofe X} :
+    Cofe (gReifiers_state rs ♯ X).
+  Proof.
+    induction rs; simpl; first apply _.
+    destruct s. apply _.
+  Qed.
+  #[export] Instance reifiers_state_inhab {n} (rs : gReifiers n) :
+    Inhabited (gReifiers_state rs ♯ unitO).
+  Proof.
+    induction rs; simpl; first apply _.
+    destruct s. apply _.
+  Qed.
+
+  Fixpoint gState_rest {m} (i : fin m) : gReifiers m → oFunctor :=
+    match i in fin m return gReifiers m → oFunctor with
+    | 0%fin => grs_S_inv (λ _, oFunctor)
+                 (λ sR rs, gReifiers_state rs)
+    | FS j => grs_S_inv (λ _, oFunctor)
+                 (λ sR rs, sReifier_state sR * gState_rest j rs)%OF
+    end.
+
+  Lemma gState_decomp' {m} (i : fin m) (rs : gReifiers m) {X} `{!Cofe X} :
+    ofe_iso (gReifiers_state rs ♯ X)
+            ((sReifier_state (rs !!! i) ♯ X) * (gState_rest i rs ♯ X))%type.
+  Proof.
+    revert i. induction rs as [|n r rs]=>i.
+    { inversion i. }
+    inv_fin i; simpl.
+    { apply iso_ofe_refl. }
+    intros i.
+    specialize (IHrs i).
+    unshelve esplit.
+    - simple refine (λne xr, let sr := ofe_iso_1 IHrs (xr.2) in
+                             (sr.1,(xr.1,sr.2))).
+      solve_proper.
+    - simple refine (λne sxr, let r' := ofe_iso_2 IHrs (sxr.1,sxr.2.2) in
+                              (sxr.2.1, r')).
+      solve_proper.
+    - intros (s & x & rest). simpl. repeat f_equiv; rewrite ofe_iso_12//.
+    - intros (x & rest). simpl. f_equiv.
+      rewrite -surjective_pairing. apply ofe_iso_21.
+  Defined.
+  Definition gState_decomp {m} (i : fin m) {rs : gReifiers m} {X} `{!Cofe X} :
+    (gReifiers_state rs ♯ X) -n> ((sReifier_state (rs !!! i) ♯ X) * (gState_rest i rs ♯ X))%type
+    := ofe_iso_1 (gState_decomp' i rs).
+  Program Definition gState_recomp {m} {i : fin m} {rs : gReifiers m} {X} `{!Cofe X} :
+    (gState_rest i rs ♯ X) -n> (sReifier_state (rs !!! i) ♯ X) -n> (gReifiers_state rs ♯ X)
+    := λne rest st, ofe_iso_2 (gState_decomp' i rs) (st, rest).
+  Solve All Obligations with solve_proper_please.
+
+  Lemma gState_decomp_recomp {m} (i : fin m) {rs : gReifiers m} {X} `{!Cofe X}
+    (σ : sReifier_state (rs !!! i) ♯ X) rest :
+    gState_decomp i (gState_recomp rest σ) ≡ (σ, rest).
+  Proof. rewrite ofe_iso_12. reflexivity. Qed.
+  Lemma gState_recomp_decomp {m} (i : fin m) {rs : gReifiers m} {X} `{!Cofe X}
+    (σ : sReifier_state (rs !!! i) ♯ X) rest fs :
+      gState_decomp i fs ≡ (σ, rest) →
+      gState_recomp rest σ ≡ fs.
+  Proof.
+    unfold gState_recomp. simpl.
+    intros <-. rewrite ofe_iso_21//.
+  Qed.
+  Opaque gState_recomp gState_decomp.
+
+  Program Definition gReifiers_re {n} (rs : gReifiers n) {X} `{!Cofe X}
+    (op : opid (gReifiers_ops rs)) :
+    (Ins (gReifiers_ops rs op) ♯ X) * (gReifiers_state rs ♯ X) -n>
+      optionO ((Outs (gReifiers_ops rs op) ♯ X) * (gReifiers_state rs ♯ X))
+    :=  λne xst,
+      let  i := projT1 op in
+      let op' := projT2 op in
+      let x := xst.1 in
+      let st := xst.2 in
+      let fs := gState_decomp i st in
+      let σ := fs.1 in
+      let rest := fs.2 in
+      let rx := sReifier_re (rs !!! i) op' (x, σ) in
+      optionO_map (prodO_map idfun (gState_recomp rest)) rx.
+  Next Obligation. solve_proper_please. Qed.
+
+  (** We can turn a collection of reifiers into a single reifier *)
+  Definition gReifiers_sReifier {n} (rs : gReifiers n) : sReifier :=
+    {| sReifier_ops := gReifiers_ops rs;
+       sReifier_state := gReifiers_state rs;
+       sReifier_re := @gReifiers_re n rs;
+    |}.
+
+  Lemma gReifiers_re_idx {n}  (i : fin n) (rs : gReifiers n)
+    {X} `{!Cofe X} (op : opid (sReifier_ops (rs !!! i)))
+    (x : Ins (sReifier_ops _ op) ♯ X)
+    (σ : sReifier_state (rs !!! i) ♯ X) (rest : gState_rest i rs ♯ X) :
+    gReifiers_re rs (existT i op) (x, gState_recomp rest σ) ≡
+      optionO_map (prodO_map idfun (gState_recomp rest))
+           (sReifier_re (rs !!! i) op (x,σ)).
+  Proof.
+    unfold gReifiers_re. cbn-[prodO_map optionO_map].
+    f_equiv; last repeat f_equiv.
+    - eapply optionO_map_proper.
+      intros [x1 x2]; simpl. f_equiv.
+      f_equiv. f_equiv.
+      rewrite gState_decomp_recomp//.
+    - rewrite gState_decomp_recomp//.
+  Qed.
+
+  Class subReifier {n} (r : sReifier) (rs : gReifiers n) :=
+    { sR_idx : fin n;
+      sR_ops :: subEff (sReifier_ops r) (sReifier_ops (rs !!! sR_idx));
+      sR_state  {X} `{!Cofe X} :
+        ofe_iso (sReifier_state r ♯ X) (sReifier_state (rs !!! sR_idx) ♯ X);
+      sR_re m {X} `{!Cofe X} (op : opid (sReifier_ops r))
+        (x : Ins (sReifier_ops _ op) ♯ X)
+        (y : Outs (sReifier_ops _ op) ♯ X)
+        (s1 s2 : sReifier_state r ♯ X) :
+        sReifier_re r op (x, s1) ≡{m}≡ Some (y, s2) →
+        sReifier_re (rs !!! sR_idx) (subEff_opid op)
+          (subEff_conv_ins x, ofe_iso_1 sR_state s1) ≡{m}≡
+          Some (subEff_conv_outs y, ofe_iso_1 sR_state s2) }.
+
+  #[global] Instance subReifier_here {n} (r : sReifier) (rs : gReifiers n) :
+    subReifier r (gReifiers_cons r rs).
+  Proof.
+    simple refine ({| sR_idx := 0%fin |}).
+    - simpl. intros. apply iso_ofe_refl.
+    - intros X ? op x y s1 s2.
+      simpl. eauto.
+  Defined.
+  #[global] Instance subReifier_there {n} (r r' : sReifier) (rs : gReifiers n) :
+    subReifier r rs →
+    subReifier r (gReifiers_cons r' rs).
+  Proof.
+    intros SR.
+    simple refine ({| sR_idx := FS sR_idx |}).
+    - simpl. intros. apply sR_state.
+    - intros X ? op x y s1 s2.
+      simpl. apply sR_re.
+  Defined.
+
+  #[local] Definition subR_op {n} {r : sReifier} {rs : gReifiers n} `{!subReifier r rs} :
+    opid (sReifier_ops r) → opid (gReifiers_ops rs).
+  Proof.
+    intros op.
+    simpl.
+    refine (existT sR_idx (subEff_opid op)).
+  Defined.
+  Definition subR_conv_state {n} {r : sReifier} {rs : gReifiers n} `{!subReifier r rs}
+    {X} `{!Cofe X}:
+    (sReifier_state r ♯ X) -n> (sReifier_state (rs !!! sR_idx) ♯ X) :=
+    ofe_iso_1 sR_state.
+  #[export] Instance subReifier_subEff {n} {r : sReifier} {rs : gReifiers n} `{!subReifier r rs} :
+    subEff (sReifier_ops r) (gReifiers_ops rs).
+  Proof.
+    simple refine {| subEff_opid := subR_op |}.
+    - intros op X ?. simpl.
+      apply subEff_ins.
+    - intros op X ?. simpl.
+      apply subEff_outs.
+  Defined.
+
+  Lemma subReifier_reify_idx {n} (r : sReifier) (rs : gReifiers n)
+    `{!subReifier r rs} {X} `{!Cofe X} (op : opid (sReifier_ops r))
+    (x : Ins (sReifier_ops _ op) ♯ X)
+    (y : Outs (sReifier_ops _ op) ♯ X)
+    (s1 s2 : sReifier_state r ♯ X) :
+        sReifier_re r op (x, s1) ≡ Some (y, s2) →
+        sReifier_re (rs !!! sR_idx) (subEff_opid op)
+          (subEff_conv_ins x, ofe_iso_1 sR_state s1) ≡
+          Some (subEff_conv_outs y, ofe_iso_1 sR_state s2).
+  Proof.
+    intros Hx. apply equiv_dist=>m.
+    apply sR_re. by apply equiv_dist.
+  Qed.
+
+  Lemma subReifier_reify {n} (r : sReifier)
+    (rs : gReifiers n) `{!subReifier r rs} {X} `{!Cofe X}
+    (op : opid (sReifier_ops r))
+    (x : Ins (sReifier_ops _ op) ♯ X) (y : Outs (sReifier_ops _ op) ♯ X)
+    (σ σ' : sReifier_state r ♯ X) (rest : gState_rest sR_idx rs ♯ X) :
+    sReifier_re r op (x,σ) ≡ Some (y, σ') →
+    gReifiers_re rs (subEff_opid op)
+      (subEff_conv_ins x, gState_recomp rest (subR_conv_state σ))
+      ≡ Some (subEff_conv_outs y, gState_recomp rest (subR_conv_state σ')).
+  Proof.
+    intros Hre.
+    eapply subReifier_reify_idx in Hre.
+    rewrite gReifiers_re_idx//.
+    rewrite Hre. simpl. reflexivity.
+  Qed.
+
+  (** Lemma for reasoning internally in iProp *)
+  Context `{!invGS_gen hlc Σ}.
+  Notation iProp := (iProp Σ).
+  Context {sz : nat}.
+  Variable (rs : gReifiers sz).
+  Notation sr := (gReifiers_sReifier rs).
+
+  Lemma reify_vis_eqI  op i k o σ σ' :
+    (gReifiers_re rs op (i,σ) ≡ Some (o,σ') ⊢@{iProp} reify sr (Vis op i k) σ ≡ (σ', Tau $ k o))%I.
+  Proof.
+    apply uPred.internal_eq_entails=>m.
+    intros H. apply reify_vis_dist. exact H.
+  Qed.
+  Lemma subReifier_reify_idxI (r : sReifier)
+    `{!subReifier r rs} {X} `{!Cofe X} (op : opid (sReifier_ops r))
+    (x : Ins (sReifier_ops _ op) ♯ X)
+    (y : Outs (sReifier_ops _ op) ♯ X)
+    (s1 s2 : sReifier_state r ♯ X) :
+        sReifier_re r op (x, s1) ≡ Some (y, s2) ⊢@{iProp}
+        sReifier_re (rs !!! sR_idx) (subEff_opid op)
+          (subEff_conv_ins x, ofe_iso_1 sR_state s1) ≡
+          Some (subEff_conv_outs y, ofe_iso_1 sR_state s2).
+  Proof.
+    apply uPred.internal_eq_entails=>m.
+    apply sR_re.
+  Qed.
+
+  Lemma subReifier_reifyI (r : sReifier)
+    `{!subReifier r rs} {X} `{!Cofe X}
+    (op : opid (sReifier_ops r))
+    (x : Ins (sReifier_ops _ op) ♯ X) (y : Outs (sReifier_ops _ op) ♯ X)
+    (σ σ' : sReifier_state r ♯ X) (rest : gState_rest sR_idx rs ♯ X) :
+    sReifier_re r op (x,σ) ≡ Some (y, σ') ⊢@{iProp}
+    gReifiers_re rs (subEff_opid op)
+      (subEff_conv_ins x, gState_recomp rest (subR_conv_state σ))
+      ≡ Some (subEff_conv_outs y, gState_recomp rest (subR_conv_state σ')).
+  Proof.
+    apply uPred.internal_eq_entails=>m.
+    intros He.
+    eapply sR_re in He.
+    rewrite gReifiers_re_idx//.
+    rewrite He. simpl. reflexivity.
+  Qed.
+
+End greifiers.
