theories/input_lang/logrel.v
@@ -378,7 +378,7 @@ Definition rs : gReifiers 1 := gReifiers_cons reify_input gReifiers_nil.
 Lemma logrel_nat_adequacy {S} (α : IT (gReifiers_ops rs)) (e : expr S) n σ σ' k :
   (∀ {Σ:gFunctors}`{H1 : !invGS Σ} `{H2: !stateG rs Σ},
       (True ⊢ logrel rs Tnat α e)%I) →
-  ssteps rs α (σ,()) (Nat n) σ' k → ∃ m σ', prim_steps e σ (Val $ Lit n) σ' m.
+  ssteps (gReifiers_sReifier rs) α (σ,()) (Nat n) σ' k → ∃ m σ', prim_steps e σ (Val $ Lit n) σ' m.
 Proof.
   intros Hlog Hst.
   pose (ϕ := λ (βv : ITV (gReifiers_ops rs)),
@@ -435,7 +435,7 @@ Qed.
 
 Theorem adequacy (e : expr []) (k : nat) σ σ' n :
   typed empC e Tnat →
-  ssteps rs (interp_expr rs e ()) (σ,()) (Nat k) σ' n →
+  ssteps (gReifiers_sReifier rs) (interp_expr rs e ()) (σ,()) (Nat k) σ' n →
   ∃ mm σ', prim_steps e σ (Val $ Lit k) σ' mm.
 Proof.
   intros Hty Hst.
